Remove length constraint on input for pure parser specs

examples/lowparse/LowParse.Impl.VLBytes.Part2.Subpart3.fst
@@ -9,7 +9,7 @@ module U16 = FStar.UInt16
 
 #set-options "--z3rlimit 16"
 
-let be_to_n_1 (b: bytes32) : Lemma
+let be_to_n_1 (b: bytes) : Lemma
   (requires (Seq.length b == 1))
   (ensures (
     Seq.length b == 1 /\
@@ -22,13 +22,13 @@ let be_to_n_1 (b: bytes32) : Lemma
 #set-options "--z3rlimit 64"
 
 let parse_bounded_integer'_3_correct_some
-  (b: bytes32)
+  (b: bytes)
 : Lemma
   (requires (Some? (parse (parse_bounded_integer' 3) b)))
   (ensures (parse (parse_bounded_integer' 3) b == parse (parse_bounded_integer 3) b))
 = assert (Some? (parse (parse_bounded_integer 3) b));
   let (Some (v, consumed)) = parse (parse_bounded_integer 3) b in
-  let b1 : bytes32 = Seq.slice b 0 3 in
+  let b1 : bytes = Seq.slice b 0 3 in
   assert (v == decode_bounded_integer 3 b1);
   E.lemma_be_to_n_is_bounded b1;
   assert (E.be_to_n b1 < pow2 24);
@@ -36,9 +36,9 @@ let parse_bounded_integer'_3_correct_some
   assert (E.be_to_n b1 < pow2 32);
   let x = U32.uint_to_t (E.be_to_n b1) in
   assert (v == x);
-  let b1l : bytes32 = Seq.slice b1 0 2 in
+  let b1l : bytes = Seq.slice b1 0 2 in
   assert (b1l == Seq.slice b 0 2);
-  let b1r : bytes32 = Seq.slice b1 2 3 in
+  let b1r : bytes = Seq.slice b1 2 3 in
   assert (E.be_to_n b1 == U8.v (Seq.last b1) + FStar.Mul.op_Star (pow2 8) (E.be_to_n b1l));
   assert (Seq.last b1r == Seq.last b1);
   be_to_n_1 b1r;
@@ -46,7 +46,7 @@ let parse_bounded_integer'_3_correct_some
   let (Some (v', consumed')) = parse (parse_bounded_integer' 3) b in  
   assert (consumed == consumed');
   let (Some (vl, _)) = parse parse_u16 b in
-  let b_ : bytes32 = Seq.slice b 2 (Seq.length b) in
+  let b_ : bytes = Seq.slice b 2 (Seq.length b) in
   let (Some (vr, _)) = parse parse_u8 b_ in
   let (Some (vp, _)) = parse (nondep_then parse_u16 parse_u8) b in
   assume (vp == (vl, vr));
@@ -67,7 +67,7 @@ let parse_bounded_integer'_3_correct_some
 #reset-options
 
 let parse_bounded_integer'_3_correct
-  (b: bytes32)
+  (b: bytes)
 : Lemma
   (parse (parse_bounded_integer' 3) b == parse (parse_bounded_integer 3) b)
 = let pv' = parse (parse_bounded_integer' 3) b in
