examples/lowparse/LowParse.Bytes.fst
@@ -5,6 +5,3 @@ module U8 = FStar.UInt8
 
 type byte = U8.byte
 type bytes = Seq.seq byte
-/// the abstract model of input is a sequence of bytes, with a limit on size so
-/// offsets always fit in a U32.t
-let bytes32 = bs:bytes{ Seq.length bs < pow2 32}
