examples/lowparse/LowParse.Impl.VLBytes.Part2.Subpart1.fst
@@ -4,7 +4,7 @@ include LowParse.Impl.VLBytes.Part1
 #set-options "--z3rlimit 32"
 
 let parse_bounded_integer'_1_correct
-  (b: bytes32)
+  (b: bytes)
 : Lemma
   (parse (parse_bounded_integer' 1) b == parse (parse_bounded_integer 1) b)
 = ()
