examples/lowparse/LowParse.Impl.VLBytes.Part2.fsti
@@ -3,6 +3,6 @@ include LowParse.Impl.VLBytes.Part1
 
 val parse_bounded_integer'_correct
   (i: integer_size)
-  (b: bytes32)
+  (b: bytes)
 : Lemma
   (parse (parse_bounded_integer' i) b == parse (parse_bounded_integer i) b)
